\documentclass[a4paper]{PRseminar}
%\usepackage{txfonts}
\usepackage{color}

\title{PR Seminar}

\author{D3 Rei Kawashima}

\inst{}
\abst{}
\setlength{\topmargin}{-10.0truemm}
\addtolength{\textheight}{0truemm}
\setlength{\oddsidemargin}{-13truemm}
\setlength{\evensidemargin}{-13truemm}
\addtolength{\textwidth}{30truemm}
\begin{document}
%\maketitle
	


\section{Linear expression of HES}
	\begin{equation}
		\Delta Q+\Delta tA\left(\frac{\partial Q}{\partial x}\right)+\Delta tB\left(\frac{\partial Q}{\partial y}\right)=0
	\end{equation}
	\begin{equation}
		Q=\left(\phi,u,v\right)^T,
		\hspace{20pt}
		A=\left(\begin{array}{ccc}
			\  & 1 & \ \\
			1  & \ & \ \\
			\  & \ & \ \\
		\end{array}\right),
		\hspace{20pt}
		B=\left(\begin{array}{ccc}
			\  & \ & 1 \\
			\ & \  & \ \\
			1 & \ &\ \\
		\end{array}\right).
	\end{equation}
	
\subsection{First-order discretization}
	\begin{equation}
		\Delta t\left(\frac{\partial E}{\partial x}\right)=
		\left(\begin{array}{c}
			\sum_{i-1}^{i+1}\left(a_k\phi_k+b_ku_k\right)  \\
			\sum_{i-1}^{i+1}\left(c_k\phi_k+d_ku_k\right)  \\
			0 \\
		\end{array}\right),
		\hspace{20pt}
		\Delta t\left(\frac{\partial F}{\partial x}\right)=
		\left(\begin{array}{c}
			\sum_{j-1}^{j+1}\left(e_k\phi_k+f_kv_k\right)  \\
			0\\
			\sum_{j-1}^{j+1}\left(g_k\phi_k+h_kv_k\right)  \\
		\end{array}\right).
	\end{equation}
	\begin{align}
		a_{i-1} =-   \frac{\Delta t}{2\Delta x}\hspace{20mm}
		a_{i  }&=\ \ \frac{\Delta t}{ \Delta x}\hspace{20mm}
		a_{i+1} =-   \frac{\Delta t}{2\Delta x}\\
		b_{i-1} =-   \frac{\Delta t}{2\Delta x}\hspace{20mm}
		b_{i  }&=\ \ 0                         \hspace{25mm}
		b_{i+1} =\ \ \frac{\Delta t}{2\Delta x}
	\end{align}
	\begin{align}
		c_{i-1} =-   \frac{\Delta t}{2\Delta x}\hspace{20mm}
		c_{i  }&=\ \ 0                         \hspace{25mm}
		c_{i+1} =\ \ \frac{\Delta t}{2\Delta x}\\
		d_{i-1} =-   \frac{\Delta t}{2\Delta x}\hspace{20mm}
		d_{i  }&=\ \ \frac{\Delta t}{ \Delta x}\hspace{20mm}
		d_{i+1} =-   \frac{\Delta t}{2\Delta x}
	\end{align}
	\begin{align}
		e_{j-1} =-   \frac{\Delta t}{2\Delta y}\hspace{20mm}
		e_{j  }&=\ \ \frac{\Delta t}{ \Delta y}\hspace{20mm}
		e_{j+1} =-   \frac{\Delta t}{2\Delta y}\\
		f_{j-1} =-   \frac{\Delta t}{2\Delta y}\hspace{20mm}
		f_{j  }&=\ \ 0                         \hspace{25mm}
		f_{j+1} =\ \ \frac{\Delta t}{2\Delta y}
	\end{align}
	\begin{align}
		g_{j-1} =-   \frac{\Delta t}{2\Delta y}\hspace{20mm}
		g_{j  }&=\ \ 0                         \hspace{25mm}
		g_{j+1} =\ \ \frac{\Delta t}{2\Delta y}\\
		h_{j-1} =-   \frac{\Delta t}{2\Delta y}\hspace{20mm}
		h_{j  }&=\ \ \frac{\Delta t}{ \Delta y}\hspace{20mm}
		h_{j+1} =-   \frac{\Delta t}{2\Delta y}
	\end{align}

	\clearpage
\subsection{Second-order discretization}
	\begin{equation}
		\Delta t\left(\frac{\partial E}{\partial x}\right)=
		\left(\begin{array}{c}
			\sum_{i-2}^{i+2}\left(a_k\phi_k+b_ku_k\right)  \\
			\sum_{i-2}^{i+2}\left(c_k\phi_k+d_ku_k\right)  \\
			0 \\
		\end{array}\right),
		\hspace{20pt}
		\Delta t\left(\frac{\partial F}{\partial x}\right)=
		\left(\begin{array}{c}
			\sum_{j-2}^{j+2}\left(e_k\phi_k+f_kv_k\right)  \\
			0\\
			\sum_{j-2}^{j+2}\left(g_k\phi_k+h_kv_k\right)  \\
		\end{array}\right).
	\end{equation}
	\begin{align}
		a_{i-2}&=\ \ \frac{\Delta t}{4\Delta x}s_{\phi1,i-1}\nonumber\\
		a_{i-1}&=-   \frac{\Delta t}{4\Delta x}\left(2+s_{\phi1,i-1}-s_{\phi2,i-1}\right)\nonumber\\
		a_{i  }&=\ \ \frac{\Delta t}{4\Delta x}\left(4-s_{\phi1,i+1}-s_{\phi2,i-1}\right)       \\
		a_{i+1}&=-   \frac{\Delta t}{4\Delta x}\left(2-s_{\phi1,i+1}+s_{\phi2,i+1}\right)\nonumber\\
		a_{i+2}&=\ \ \frac{\Delta t}{4\Delta x}s_{\phi2,i+1}\nonumber\\\\
		b_{i-2}&=\ \ \frac{\Delta t}{4\Delta x}s_{u1,i-1}\nonumber\\
		b_{i-1}&=-   \frac{\Delta t}{4\Delta x}\left(2+s_{u1,i-1}-s_{u2,i-1}+2s_{u1,i}\right)\nonumber\\
		b_{i  }&=\ \ \frac{\Delta t}{4\Delta x}\left(-s_{u2,i-1}+2s_{u1,i}-2s_{u2,i}+s_{u1,i+1}\right)       \\
		b_{i+1}&=\ \ \frac{\Delta t}{4\Delta x}\left(2-s_{u1,i+1}+s_{u2,i+1}+2s_{u2,i}\right)\nonumber\\
		b_{i+2}&=-   \frac{\Delta t}{4\Delta x}s_{u2,i+1}\nonumber
	\end{align}
	\clearpage
	\begin{align}
		c_{i-2}&=\ \ \frac{\Delta t}{4\Delta x}s_{\phi1,i-1}\nonumber\\
		c_{i-1}&=-   \frac{\Delta t}{4\Delta x}\left(2+s_{\phi1,i-1}-s_{\phi2,i-1}+2s_{\phi1,i}\right)\nonumber\\
		c_{i  }&=\ \ \frac{\Delta t}{4\Delta x}\left(-s_{\phi2,i-1}+2s_{\phi1,i}-2s_{\phi2,i}+s_{\phi1,i+1}\right)       \\
		c_{i+1}&=\ \ \frac{\Delta t}{4\Delta x}\left(2-s_{\phi1,i+1}+s_{\phi2,i+1}+2s_{\phi2,i}\right)\nonumber\\
		c_{i+2}&=-   \frac{\Delta t}{4\Delta x}s_{\phi2,i+1}\nonumber\\\\
		d_{i-2}&=\ \ \frac{\Delta t}{4\Delta x}s_{u1,i-1}\nonumber\\
		d_{i-1}&=-   \frac{\Delta t}{4\Delta x}\left(2+s_{u1,i-1}-s_{u2,i-1}\right)\nonumber\\
		d_{i  }&=\ \ \frac{\Delta t}{4\Delta x}\left(4-s_{u1,i+1}-s_{u2,i-1}\right)       \\
		d_{i+1}&=-   \frac{\Delta t}{4\Delta x}\left(2-s_{u1,i+1}+s_{u2,i+1}\right)\nonumber\\
		d_{i+2}&=\ \ \frac{\Delta t}{4\Delta x}s_{u2,i+1}\nonumber\\\\
		e_{j-2}&=\ \ \frac{\Delta t}{4\Delta y}t_{\phi1,j-1}\nonumber\\
		e_{j-1}&=-   \frac{\Delta t}{4\Delta y}\left(2+t_{\phi1,j-1}-t_{\phi2,j-1}\right)\nonumber\\
		e_{j  }&=\ \ \frac{\Delta t}{4\Delta y}\left(4-t_{\phi1,j+1}-t_{\phi2,j-1}\right)       \\
		e_{j+1}&=-   \frac{\Delta t}{4\Delta y}\left(2-t_{\phi1,j+1}+t_{\phi2,j+1}\right)\nonumber\\
		e_{j+2}&=\ \ \frac{\Delta t}{4\Delta y}t_{\phi2,j+1}\nonumber\\
	\end{align}
	\clearpage
	\begin{align}
		f_{j-2}&=\ \ \frac{\Delta t}{4\Delta y}t_{v1,j-1}\nonumber\\
		f_{j-1}&=-   \frac{\Delta t}{4\Delta y}\left(2+t_{v1,j-1}-t_{v2,j-1}+2t_{v1,j}\right)\nonumber\\
		f_{j  }&=\ \ \frac{\Delta t}{4\Delta y}\left(-t_{v2,j-1}+2t_{v1,j}-2t_{v2,j}+t_{v1,j+1}\right)       \\
		f_{j+1}&=\ \ \frac{\Delta t}{4\Delta y}\left(2-t_{v1,j+1}+t_{v2,j+1}+2t_{v2,j}\right)\nonumber\\
		f_{j+2}&=-   \frac{\Delta t}{4\Delta y}t_{v2,j+1}\nonumber \\\\
		g_{j-2}&=\ \ \frac{\Delta t}{4\Delta y}t_{\phi1,j-1}\nonumber\\
		g_{j-1}&=-   \frac{\Delta t}{4\Delta y}\left(2+t_{\phi1,j-1}-t_{\phi2,j-1}+2t_{\phi1,j}\right)\nonumber\\
		g_{j  }&=\ \ \frac{\Delta t}{4\Delta y}\left(-t_{\phi2,j-1}+2t_{\phi1,j}-2t_{\phi2,j}+t_{\phi1,j+1}\right)       \\
		g_{j+1}&=\ \ \frac{\Delta t}{4\Delta y}\left(2-t_{\phi1,j+1}+t_{\phi2,j+1}+2t_{\phi2,j}\right)\nonumber\\
		g_{j+2}&=-   \frac{\Delta t}{4\Delta y}t_{\phi2,j+1}\nonumber\\\\
		h_{j-2}&=\ \ \frac{\Delta t}{4\Delta y}t_{v1,j-1}\nonumber\\
		h_{j-1}&=-   \frac{\Delta t}{4\Delta y}\left(2+t_{v1,j-1}-t_{v2,j-1}\right)\nonumber\\
		h_{j  }&=\ \ \frac{\Delta t}{4\Delta y}\left(4-t_{v1,j+1}-t_{v2,j-1}\right)       \\
		h_{j+1}&=-   \frac{\Delta t}{4\Delta y}\left(2-t_{v1,j+1}+t_{v2,j+1}\right)\nonumber\\
		h_{j+2}&=\ \ \frac{\Delta t}{4\Delta y}t_{v2,j+1}\nonumber
	\end{align}
\end{document}

